Values.v
@@ -2,10 +2,10 @@ Require Import SLFun.Util.
 
 
 Definition ptr : Type := nat.
+Definition NULL : ptr := O.
 
 Definition memdata : Type := nat.
 
-(* TODO: only for non null pointers *)
 Definition mem : Type := ptr -> memdata.
 
 Module Mem.
@@ -13,14 +13,8 @@ Module Mem.
 
   Definition read (m : t) (p : ptr) : memdata := m p.
 
-  (* TODO? Stdlib *)
-  Fixpoint ptr_eq (p0 p1 : ptr) {struct p0} : {p0 = p1}+{p0<>p1}.
-  Proof.
-    case p0 as [|p0], p1 as [|p1].
-    2,3:right; discriminate 1.
-    - left; reflexivity.
-    - case (ptr_eq p0 p1); [left|right]; congruence.
-  Defined.
+  Definition ptr_eq (p0 p1 : ptr) : {p0 = p1}+{p0<>p1}.
+  Proof. decide equality. Defined.
 
   Definition write (m : t) (p : ptr) (x : memdata) : t :=
     fset ptr_eq p x m.
